lemmes d'alpha-équivalence sur les AST

theories/ast.v
@@ -3,7 +3,7 @@ Require Import ssreflect ssrfun ssrbool ssrnat eqtype choice seq fintype.
 From MathComp
 Require Import bigop  finfun finset generic_quotient perm tuple fingroup.
 From Nominal
-Require Import finmap finsfun finperm nominal ast.
+Require Import finmap finsfun finperm nominal.
 
 Require Import Program.
 
@@ -18,6 +18,52 @@ Local Open Scope quotient_scope.
 
 Import Key.Exports.
 
+Section Utils.
+
+Definition maxlist l := foldr maxn 0 l.
+
+Lemma maxlist_leqP l n : reflect (forall x, x \in l -> x <= n)
+                                 (maxlist l <= n).
+Proof.
+apply: (iffP idP); elim: l => //.
+  move => m l IHl /=.  
+  rewrite geq_max => /andP [m_leq_n maxl_leq_n] p.
+  rewrite in_cons => /orP. case.
+    by move/eqP ->.
+  exact: IHl.
+move => m l IHl Hml /=.
+rewrite geq_max. apply/andP; split.
+  exact/Hml/mem_head.
+apply IHl => p pl.
+apply Hml. by rewrite in_cons pl orbT.
+Qed.
+
+Lemma in_maxlist l x : x \in l -> x <= maxlist l.
+Proof.
+elim: l => //= a l IHl.
+rewrite in_cons => /orP. case.
+  move/eqP ->. by rewrite leq_maxl.
+move/IHl => x_leq_maxl. apply (@leq_trans (maxlist l)) => //.
+by rewrite leq_maxr.
+Qed.
+
+Fixpoint all2 {A : eqType} (p : A -> A -> bool) (l1 l2 : seq A) :=
+  match l1, l2 with
+    |[::], [::] => true
+    |a::q, b::r => (p a b) && all2 p q r
+    |_, _ => false
+  end.
+
+Lemma eq_in_all2 {A : eqType} (s1 s2 : seq A) (p1 p2 : A -> A -> bool) : 
+  {in s1 & s2, p1 =2 p2} -> all2 p1 s1 s2  = all2 p2 s1 s2.
+Proof.
+elim: s1 s2. by case.
+move => a1 s1 IHl. case => // a2 s2 p1_eq_p2 /=. 
+rewrite p1_eq_p2 ?mem_head // IHl //.
+move => x1 x2 x1s1 x2s2. apply p1_eq_p2;
+by rewrite inE (x1s1, x2s2) orbT.
+Qed.
+
 Section ASTDef.
 
 Variables (node_label : Type) (leaf_type: nominalType atom).
@@ -25,7 +71,7 @@ Variables (node_label : Type) (leaf_type: nominalType atom).
 Inductive rAST := 
 |rLeaf of leaf_type
 |rCons of node_label & seq rAST
-|rBinderCons of node_label * atom & seq rAST.
+|rBinderCons of node_label & atom & seq rAST.
 
 
 (* TODO : encodage des rAST *)
@@ -48,7 +94,7 @@ Definition rAST_better_rect T IH_leaf IH_cons IH_bcons :=
   match t with
   | rLeaf x => IH_leaf x
   | rCons c f0 => IH_cons c f0 (result_list f0)
-  | rBinderCons (c, x) f0 => IH_bcons (c,x) f0 (result_list f0) 
+  | rBinderCons c x f0 => IH_bcons (c,x) f0 (result_list f0) 
     end.
 
 Lemma rAST_better_ind_subproof (P : rAST -> Prop) (f : seq rAST): 
@@ -68,26 +114,35 @@ Definition rAST_better_ind P IH_leaf IH_cons IH_bcons :=
   match t with
   | rLeaf x => IH_leaf x
   | rCons c f0 => IH_cons c f0 (rAST_better_ind_subproof (iter_conj f0))
-  | rBinderCons (c, x) f0 => IH_bcons (c,x) f0 (rAST_better_ind_subproof (iter_conj f0))
+  | rBinderCons c x f0 => IH_bcons c x f0 (rAST_better_ind_subproof (iter_conj f0))
     end.
 
-Definition rAST_depth : rAST -> nat.
-apply/rAST_better_rect => [_|_ _ l|_ _ l].
-  - exact: 0. 
-  - exact: (foldr maxn 0 l).+1.
-  - exact: (foldr maxn 0 l).+1.
-Defined.
+Variable (s : seq nat).
+
+Fixpoint rAST_depth (t : rAST) : nat :=
+  match t with
+    |rLeaf _ => 0
+    |rCons _ l => (maxlist (map rAST_depth l)).+1
+    |rBinderCons _ _ l => (maxlist (map rAST_depth l)).+1
+  end.
+
+(* Lemma rAST_size_ind (P : rAST -> Prop) : *)
+(*   (forall (x : leaf_type), P (rLeaf x)) -> *)
+(*   (forall W,  (forall W', rAST_depth W' <= rAST_depth W -> P W') -> P W) -> *)
+(*   forall W, P W. *)
+(* Admitted. *)
+
 
 Fixpoint rAST_act (π : {finperm atom}) (t : rAST) :=
   match t with
     |rLeaf u => rLeaf (π \dot u)
     |rCons c l => rCons c [seq (rAST_act π u) | u <- l]
-    |rBinderCons (c, x) l => rBinderCons (c, π x) [seq (rAST_act π u) | u <- l]
+    |rBinderCons c x l => rBinderCons c (π x) [seq (rAST_act π u) | u <- l]
   end.
 
 Lemma rAST_act1 : rAST_act (1 atom) =1 id.
 Proof. 
-elim/rAST_better_ind => [x|c l IHl|[c x] l IHl] /=.
+elim/rAST_better_ind => [x|c l IHl|c x l IHl] /=.
   - by rewrite act1.
   - by rewrite map_id_in //.
   - by rewrite finsfun1 map_id_in.
@@ -96,7 +151,7 @@ Qed.
 Lemma rAST_actM π π' (t : rAST) : 
   rAST_act (π * π') t = rAST_act π (rAST_act π' t).
 Proof.
-elim/rAST_better_ind :t => [x|c l IHl|[c x] l IHl] /=.
+elim/rAST_better_ind :t => [x|c l IHl|c x l IHl] /=.
   - by rewrite actM.
   - congr rCons. rewrite -map_comp. 
     apply eq_in_map => t /=. exact: IHl.
@@ -132,7 +187,7 @@ Qed.
 Lemma rAST_act_id (π : {finperm atom}) (t : rAST) :
      (forall a : atom, a \in rAST_support t -> π a = a) -> rAST_act π t = t.
 Proof.
-elim/rAST_better_ind : t => [x|c l IHl|[c x] l IHl] Hsupp /=.
+elim/rAST_better_ind : t => [x|c l IHl|c x l IHl] Hsupp /=.
   - by rewrite act_id.
   - rewrite map_id_in // => t t_in_l.
     apply IHl => // a a_supp_t.
@@ -156,24 +211,112 @@ Canonical rAST_nominalType (node_label : Type) (leaf_type : nominalType atom) :=
     (@rAST_choiceType node_label leaf_type) 
     (@rAST_nominal_mixin node_label leaf_type).
 
+Section Depth.
+
+Variables (node_label : Type) (leaf_type : nominalType atom).
+  
+Lemma depth_cons_leq {c} {l} {n} : 
+  rAST_depth (rCons c l) <= n.+1 -> 
+  all (fun t : rAST node_label leaf_type => rAST_depth t <= n) l.
+Proof.
+rewrite ltnS => /maxlist_leqP Hl.
+apply/allP => x xl. 
+exact/Hl/map_f.
+Qed.
+
+Lemma depth_perm (π : {finperm atom}) (t : rAST node_label leaf_type) : 
+rAST_depth (π \dot t) = rAST_depth t.
+Proof. 
+elim/rAST_better_ind: t => [x|? l ihl|? ? l ihl] //=. 
+all: apply eq_S; congr maxlist; rewrite -map_comp.
+all: apply eq_in_map => t tl /=.
+all: exact: ihl.
+Qed.
+
+End Depth.
+
+Section WellFormedness.
+
+Variables (node_label : Type) (leaf_type : nominalType atom) (arity : node_label -> nat).
+
+Fixpoint wf (t : rAST node_label leaf_type) : bool :=
+  match t with
+    |rLeaf _ => true
+    |rCons c l => (size l == arity c) && (all wf l)
+    |rBinderCons c _ l => (size l == arity c) && (all wf l)
+  end.
+
+Definition wf_rAST := sig_subType wf.
+
+End WellFormedness.
+
 Section AlphaEquivalence.
 
-Variables (node_label : eqType) (leaf_type : nominalType atom).
+Variables (node_label : eqType) 
+          (leaf_type : nominalType atom) 
+          (arity : node_label -> nat).
 
 Fixpoint alpha_rec (n : nat) (W1 W2 : rAST node_label leaf_type) :=
   match n, W1, W2 with
     |_, rLeaf x, rLeaf y => x == y
     |S n, rCons c1 children1, rCons c2 children2 => 
-     (c1 == c2) && (all (fun z => alpha_rec n z.1 z.2) (zip children1 children2))
-    |S n, rBinderCons (c1, x) children1, rBinderCons (c2, y) children2 =>
-     (c1 == c2) && (let z := fresh_in (x, children1, y, children2) in
-                    all 
-                      (fun w => alpha_rec n (swap x z \dot w.1) (swap y z \dot w.2))
-                      (zip children1 children2))
+     (c1 == c2) && 
+     (all2 (alpha_rec n) children1 children2)
+    |S n, rBinderCons c1 x children1, rBinderCons c2 y children2 =>
+     (c1 == c2) && 
+     (let z := fresh_in (x, children1, y, children2) in
+                    all2
+                      (fun w1 w2 => alpha_rec n (swap x z \dot w1) (swap y z \dot w2))
+                      children1
+                      children2)
     |_, _,_ => false
   end.
 
 Definition alpha W1 W2 := alpha_rec (rAST_depth W1) W1 W2.     
+
+Lemma alpha_recE n (W1 W2 : rAST node_label leaf_type ) : 
+  (rAST_depth W1 <= n) -> 
+  alpha_rec n W1 W2 = alpha W1 W2.
+Proof.
+rewrite /alpha; move: {-2}n (leqnn n).
+elim: n W1 W2 => // [|n ihn] [x|c1 l1|c1 x1 l1] [y|c2 l2|c2 x2 l2] [|m] //.
+all: rewrite ltnS => m_leq_n /(@depth_cons_leq _ _ _) /allP IHl1 /=.  
+all: apply andb_id2l => _. 
+all: apply eq_in_all2 => t1 t2 t1l2 t2l2.
+  - rewrite !ihn //; last exact: IHl1.
+    apply/maxlist_leqP => r /mapP [t] tl1 ->. 
+    apply (@leq_trans m) => //. exact: IHl1.
+  exact/in_maxlist/map_f.
+  - rewrite !ihn //; last rewrite depth_perm; last exact: IHl1.
+    apply/maxlist_leqP => r /mapP [t] tl1 ->. 
+    apply (@leq_trans m) => //. exact: IHl1.
+  rewrite depth_perm. exact/in_maxlist/map_f.
+Qed.
+
+Lemma alpha_LeafE (x y : leaf_type) : 
+  alpha (rLeaf node_label x) (rLeaf node_label y) = (x == y).
+Proof. by rewrite /alpha. Qed.
+
+Lemma alpha_ConsE (c1 c2 : node_label) l1 l2 : 
+  alpha (rCons c1 l1) (rCons c2 l2) = (c1 == c2) && all2 alpha l1 l2.
+Proof. 
+rewrite/alpha /=. 
+apply andb_id2l => _. apply eq_in_all2 => t1 t2 ? ?.
+rewrite alpha_recE //. 
+exact/in_maxlist/map_f.
+Qed.
+
+Lemma alpha_BinderConsE (c1 c2 : node_label) x1 x2 l1 l2  : 
+  alpha (rBinderCons c1 x1 l1) (rBinderCons c2 x2 l2) = 
+  (c1 == c2) &&
+  let z := fresh_in (x1,l1,x2,l2) in
+  all2 (fun w1 w2 => alpha (swap x1 z \dot w1) (swap x2 z \dot w2)) l1 l2.
+Proof. 
+rewrite /alpha /=. 
+apply andb_id2l => _. apply eq_in_all2 => t1 t2 ? ?.
+rewrite alpha_recE // depth_perm.
+exact/in_maxlist/map_f.
+Qed.
 
 End AlphaEquivalence.
 
